Machinery for stdpp maps

theories/Map.v
@@ -3,7 +3,7 @@ Require Import Program.
 
 Definition dependent (K : Type) (V : K → Type) : Type := ∀ k : K, V k.
 
-Definition rebind {K : Type} {V : K → Type} `{EqDecision K} : 
+Definition insert {K : Type} {V : K → Type} `{EqDecision K} : 
   ∀ k : K, V k → dependent K V → dependent K V.
 Proof.
   intros k v m k'. unfold EqDecision in *. destruct (decide (k = k')).
@@ -11,24 +11,26 @@ Proof.
   - exact (m k').
 Defined.
 
-Notation "m { k ↦ v }" := (rebind k v m) (at level 80).
-
 Definition lookup {K : Type} {V : K → Type} `{EqDecision K} (k : K) (m : dependent K V) : V k := m k.
 
-Theorem lookup_rebind_same {K : Type} {V : K → Type} `{EqDecision K} (k : K) (v : V k) (m : dependent K V) : 
-  rebind k v m k = v.
+Theorem lookup_insert {K : Type} {V : K → Type} `{EqDecision K} (k : K) (v : V k) (m : dependent K V) : 
+  insert k v m k = v.
 Proof.
   destruct (decide (k = k)); cbv; 
   destruct (EqDecision0 k k); intuition.
   dependent destruction e0. reflexivity.
 Qed.
 
-Theorem lookup_rebind_diff {K : Type} {V : K → Type} `{EqDecision K} (k k' : K) (v : V k) (m : dependent K V) 
-  : k ≠ k' → rebind k v m k' = lookup k' m.
+Theorem lookup_insert_ne {K : Type} {V : K → Type} `{EqDecision K} (k k' : K) (v : V k) (m : dependent K V) 
+  : k ≠ k' → insert k v m k' = lookup k' m.
 Proof.
-  intros. unfold lookup, rebind. now destruct (decide (k = k')).
+  intros. unfold lookup, insert. now destruct (decide (k = k')).
 Qed.
 
 Definition t (K V : Type) := dependent K (λ _, V).
+
+Instance map_insert K `{EqDecision K} V : Insert K V (t K V) := insert.
+
+Instance map_lookup_total K `{EqDecision K} V : LookupTotal K V (t K V) := lookup.
 
 Definition with_default {K V : Type} (d : V) : t K V := λ _, d.
